\documentclass[]{article}
\usepackage{amsmath}

%opening
\title{}
\author{}

\begin{document}

\maketitle

\begin{abstract}

\end{abstract}

\section{A}\label{sec:a}
\[B\rightarrow A\Leftrightarrow\neg(B\land\neg A)\]
$A\to(B\rightarrow A)\Leftrightarrow\neg(A\wedge\lnot\neg(B\land\neg A))\Leftrightarrow\neg(A\land\lnot A\wedge B)$
\[\O\models A\to(B\rightarrow A)\]
\(A\land A\rightarrow C\Leftrightarrow A\wedge\lnot(A\land\neg C)\Leftrightarrow A\wedge(\neg A\vee C)\Leftrightarrow A\land\neg A\lor A\land C\Leftrightarrow A\wedge C\vdash C\)
\[A\wedge A\to C\vdash C\]
\(A\Leftrightarrow A\land(A\rightarrow(B\rightarrow A))\vdash B\to A\)
\[A\vdash B\to A\]
$\neg A\to\lnot B\Leftrightarrow\neg(\neg A\wedge B)\Leftrightarrow B\to A$
\[\lnot A \to \neg B\Leftrightarrow B \rightarrow A\]
$A\to(B\to C)\Leftrightarrow A\to\neg(B\wedge\neg C)\Leftrightarrow\neg(A\wedge(B\wedge\neg C))\Leftrightarrow\neg A\vee(\neg B\vee C)\Leftrightarrow\neg A\vee\neg B\vee C\newline$
\((A\to B)\to(A\to C)\Leftrightarrow\lnot(A\land\lnot B)\to\lnot(A\land\lnot C)\Leftrightarrow\lnot(\lnot(A\land\lnot B)\land(A\land\lnot C))\Leftrightarrow(A\land\lnot B)\lor\lnot(A\land\lnot C)\Leftrightarrow(A\land\lnot B)\lor(\lnot A\lor C)\Leftrightarrow\lnot B\lor\lnot A\lor C\)
\begin{gather*}
    A\to(B\to C)\Leftrightarrow(A\to B)\to(A\to C)\\
    P\leftrightarrow Q\Leftrightarrow P\land Q\vee\neg P\wedge\lnot Q\\
\end{gather*}
\end{document}
